Add proofs for GM enc/dec impl

code/experimental/he/Hacl.Impl.HE.GM.fst
@@ -14,11 +14,15 @@ open Lib.Math.Algebra
 open Hacl.Impl.Bignum
 
 module S = Hacl.Spec.HE.GM
+module M = Lib.Math.Algebra
 
 // max 2^14 bits
 type bn_len_s = s:bn_len{v s <= 256}
 
-val to_fe:
+
+#reset-options "--z3rlimit 50 --max_fuel 0 --max_ifuel 0"
+
+val to_fe_:
      #nLen:bn_len_s
   -> n:lbignum nLen
   -> a:lbignum nLen
@@ -31,29 +35,61 @@ val to_fe:
     (ensures fun h0 _ h1 ->
        modifies1 res h0 h1 /\
        as_snat h1 res = to_fe #(as_snat h0 n) (as_snat h0 a))
-let to_fe #nLen n a res = bn_remainder a n res
+let to_fe_ #nLen n a res = bn_remainder a n res
+
+
+inline_for_extraction
+val conv_one_zero_to_int:
+     #nLen:bn_len_s
+  -> x:lbignum nLen
+  -> Stack Int32.t
+    (requires fun h -> live h x /\ (as_snat h x = 1 \/ as_snat h x = 0))
+    (ensures fun h0 b h1 -> h0 == h1 /\ Int32.v b = as_snat h1 x)
+let conv_one_zero_to_int #nLen x =
+  let h = FStar.HyperStack.ST.get () in
+  let b = if eq_u64 (x.(0ul)) (uint 0) then 0l else 1l in
+
+  let l (): Lemma (Int32.v b = as_snat h x) = begin
+//    let r = as_snat h x in
+//    assert (r = 0 ==> x.(0ul) = 0uL);
+    admit() // How to combine effects?
+    end in
+
+  l ();
+
+  b
+
 
 val leg_symbol:
      #nLen:bn_len_s
-  -> a:lbignum nLen
   -> p:lbignum nLen
   -> p_min_one:lbignum nLen
   -> p_min_one_half:lbignum nLen
+  -> a:lbignum nLen
   -> Stack Int32.t
     (requires fun h ->
        live h a /\ live h p /\ live h p_min_one /\ live h p_min_one_half /\
        disjoint a p /\
        as_snat h p > 1 /\
+       isprm (as_snat h p) /\
        as_snat h p_min_one = as_snat h p - 1 /\
        as_snat h p_min_one_half = as_snat h p_min_one / 2)
-    (ensures  fun h0 _ h1 ->
-       live h1 a /\ live h1 p /\ modifies0 h0 h1)
-let leg_symbol #nLen a p p_min_one p_min_one_half =
+    (ensures fun h0 b h1 ->
+       live h1 a /\ live h1 p /\ modifies0 h0 h1 /\
+       Int32.v b = S.leg_symbol (as_snat h0 a) (as_snat h0 p)
+       )
+let leg_symbol #nLen p p_min_one p_min_one_half a =
   push_frame ();
   let tmp = create nLen (uint 0) in
   bn_modular_exp p a p_min_one_half tmp;
-  let res = if bn_is_equal p_min_one tmp then (-1l)
-            else (if eq_u64 (tmp.(0ul) &. uint 1) (uint 1) then 1l else 0l) in
+  let h = FStar.HyperStack.ST.get () in
+
+  let res = if bn_is_equal p_min_one tmp then (-1l) else begin
+              S.is_leg_symbol_raw (as_snat h p) (as_snat h a);
+              assert (let res = as_snat h tmp in res = 0 \/ res = 1);
+              conv_one_zero_to_int tmp
+            end in
+
   pop_frame ();
   res
 
@@ -62,22 +98,51 @@ val encrypt:
      #nLen:bn_len_s
   -> n:lbignum nLen
   -> y:lbignum nLen
-  -> m:bool
   -> r:lbignum nLen
+  -> msg:bool
   -> res:lbignum nLen
   -> Stack unit
     (requires fun h ->
        live h n /\ live h y /\ live h r /\ live h res /\
        disjoint n res /\ disjoint y res /\ disjoint r res /\
-       as_snat h n > 1)
+       (let n' = as_snat h n in
+       let r' = as_snat h r in
+       let y' = as_snat h y in
+       n' > 1 /\
+       y' < n' /\
+       r' < n' /\ sqr #n' r' > 0 /\ sqr #n' r' *% y' > 0))
     (ensures fun h0 _ h1 ->
        live h1 n /\ live h1 y /\ live h1 r /\ live h1 res /\
-       modifies1 res h0 h1)
-let encrypt #nLen n y m r res =
-  if m then bn_modular_mul n r r res else begin
+       modifies1 res h0 h1 /\
+       as_snat h1 res = S.encrypt_minimal (as_snat h0 n) (as_snat h0 y) (as_snat h0 r) msg)
+let encrypt #nLen n y r msg res =
+  if not msg then bn_modular_mul n r r res else begin
     push_frame ();
     let r' = create nLen (uint 0) in
-    bn_modular_mul n r r res;
+    bn_modular_mul n r r r';
     bn_modular_mul n r' y res;
     pop_frame ()
   end
+
+
+val decrypt:
+     #nLen:bn_len_s
+  -> p:lbignum nLen
+  -> p_min_one:lbignum nLen
+  -> p_min_one_half:lbignum nLen
+  -> c:lbignum nLen
+  -> Stack bool
+    (requires fun h ->
+       live h p /\ live h p_min_one /\ live h p_min_one_half /\ live h c /\
+       disjoint c p /\
+       as_snat h c > 0 /\
+       as_snat h p > 1 /\
+       isprm (as_snat h p) /\
+       as_snat h p_min_one = as_snat h p - 1 /\
+       as_snat h p_min_one_half = as_snat h p_min_one / 2)
+    (ensures fun h0 b h1 -> modifies0 h0 h1 /\
+      (let c' = as_snat h0 c in
+       b = S.decrypt_minimal (as_snat h0 p) c'))
+let decrypt #nLen p p_min_one p_min_one_half c =
+  let v = leg_symbol p p_min_one p_min_one_half c in
+  if v = 1l then false else true
